deps/poulet4/lib/P4automata/NtupleProofs.v
@@ -1,4 +1,5 @@
 Require Import Coq.Lists.List.
+Require Import Coq.Program.Equality.
 
 Require Import Poulet4.FinType.
 Require Import Poulet4.TypeNeq.
@@ -121,4 +122,240 @@ Proof.
   destruct (PeanoNat.Nat.eq_dec n m); auto.
   exfalso.
   eapply n_tuple_diff_neq; eauto.
+Qed.
+
+Lemma t2l_n_eq:
+forall n m (ys : n_tuple bool m) (xs : n_tuple bool n),
+  t2l xs = t2l ys ->
+  n = m.
+Proof.
+  intros.
+  pose proof (t2l_len n xs).
+  pose proof (t2l_len m ys).
+  congruence.
+Qed.
+
+Lemma t2l_eq:
+  forall n m (ys : n_tuple bool m) (xs : n_tuple bool n),
+    t2l xs = t2l ys ->
+    xs ~= ys.
+Proof.
+  intros.
+  pose proof (t2l_n_eq _ _ _ _ H).
+  subst m.
+  cut (xs = ys).
+  {
+    intros.
+    subst.
+    reflexivity.
+  }
+  induction n; cbn in *; destruct xs, ys; cbn in *.
+  - reflexivity.
+  - assert (b = b0).
+    {
+      apply f_equal with (f := (fun l => (@last bool) l false)) in H.
+      erewrite !last_last in H.
+      congruence.
+    }
+    subst b0.
+    apply app_inv_tail in H.
+    apply IHn in H.
+    congruence.
+Qed.
+
+Lemma eq_t2l:
+  forall n m (ys : n_tuple bool m) (xs : n_tuple bool n),
+    xs ~= ys ->
+    t2l xs = t2l ys.
+Proof.
+  intros.
+  inversion H.
+  assert (n = m) by auto using n_tuple_inj.
+  subst m.
+  rewrite H.
+  reflexivity.
+Qed.
+
+Lemma inv_jmeq_size:
+  forall n (xs: n_tuple bool n) m (ys: n_tuple bool m),
+    xs ~= ys ->
+    n = m.
+Proof.
+  intros.
+  eapply n_tuple_inj.
+  now inversion H.
+Qed.
+
+Lemma n_tuple_cons_inj_r:
+  forall n m (xs: n_tuple bool n) x (ys: n_tuple bool m) y,
+    n_tuple_cons xs x ~= n_tuple_cons ys y ->
+    xs ~= ys /\ x = y.
+Proof.
+  induction n; intros.
+  - destruct m.
+    + simpl_JMeq.
+      destruct xs, ys.
+      cbn in *.
+      intuition congruence.
+    + exfalso.
+      apply inv_jmeq_size in H.
+      Lia.lia.
+  - destruct m, xs; destruct ys.
+    + exfalso.
+      apply inv_jmeq_size in H.
+      Lia.lia.
+    + pose proof (inv_jmeq_size _ _ _ _ H).
+      assert (n = m) by Lia.lia.
+      subst m.
+      simpl_JMeq.
+      simpl in *.
+      inversion H.
+      subst b0.
+      pose proof (IHn _ n0 x n1 y ltac:(rewrite H2; reflexivity)).
+      destruct H1.
+      split; [|auto].
+      rewrite H1.
+      reflexivity.
+Qed.
+
+Lemma slice_proper:
+  forall hi lo n m (xs: n_tuple bool n) (ys: n_tuple bool m),
+    xs ~= ys ->
+    n_tuple_slice hi lo xs ~= n_tuple_slice hi lo ys.
+Proof.
+  intros hi lo n m xs ys Heq.
+  assert (n = m)
+    by (eapply inv_jmeq_size; eauto).
+  revert Heq.
+  revert xs ys.
+  subst m.
+  intros.
+  rewrite Heq.
+  reflexivity.
+Qed.
+
+Lemma concat_proper:
+  forall n1 m1 (xs1: n_tuple bool n1) (ys1: n_tuple bool m1)
+    n2 m2 (xs2: n_tuple bool n2) (ys2: n_tuple bool m2),
+    xs1 ~= xs2 ->
+    ys1 ~= ys2 ->
+    n_tuple_concat xs1 ys1 ~= n_tuple_concat xs2 ys2.
+Proof.
+  intros.
+  assert (n1 = n2) by (eapply inv_jmeq_size; eauto).
+  assert (m1 = m2) by (eapply inv_jmeq_size; eauto).
+  revert H H0.
+  revert xs2 ys2.
+  revert xs1 ys1.
+  subst n2.
+  subst m2.
+  intros.
+  rewrite H.
+  rewrite H0.
+  reflexivity.
+Qed.
+
+Lemma t2l_proper:
+  forall n m (xs: n_tuple bool n) (ys: n_tuple bool m),
+    xs ~= ys ->
+    t2l xs = t2l ys.
+Proof.
+  intros.
+  inversion H.
+  apply n_tuple_inj in H1.
+  subst n.
+  apply JMeq_eq in H.
+  congruence.
+Qed.
+
+Lemma pair_proper:
+  forall A B C D (a: A) (b: B) (c: C) (d: D),
+    a ~= b ->
+    c ~= d ->
+    (a, c) ~= (b, d).
+Proof.
+  intros.
+  inversion H.
+  inversion H0.
+  subst.
+  reflexivity.
+Qed.
+
+Lemma concat'_snoc:
+  forall n m (xs: n_tuple bool n) x (ys: n_tuple bool m),
+    n_tuple_concat' ((xs, x): n_tuple bool (S n)) ys ~= n_tuple_concat' xs (n_tuple_cons ys x).
+Proof.
+  induction m; intros.
+  - auto.
+  - destruct ys.
+    change (n_tuple_concat' ((xs, x): n_tuple bool (S n)) ((n0, b): n_tuple bool (S m)))
+      with (n_tuple_concat' ((xs, x): n_tuple bool (S n)) n0, b).
+    simpl ((xs, x) : _).
+    specialize (IHm xs x n0).
+    eapply JMeq_trans with (y:=(n_tuple_concat' xs (n_tuple_cons n0 x), b)).
+    apply pair_proper.
+    eapply IHm.
+    auto.
+    reflexivity.
+Qed.
+
+Lemma t2l_concat':
+  forall n m (xs: n_tuple bool n) (ys: n_tuple bool m),
+    t2l (n_tuple_concat' xs ys) = t2l xs ++ t2l ys.
+Proof.
+  induction n; intros.
+  - simpl in *.
+    assert (@n_tuple_concat' _ O m tt ys ~= ys)
+      by (apply (concat'_emp _ m ys); auto).
+    apply t2l_proper in H.
+    destruct xs.
+    congruence.
+  - destruct xs as [xs x].
+    simpl in *.
+    assert (n_tuple_concat' ((xs, x): n_tuple bool (S n)) ys
+            ~= n_tuple_concat' xs (n_tuple_cons ys x))
+      by eapply concat'_snoc.
+    apply t2l_proper in H.
+    rewrite H.
+    rewrite app_assoc_reverse.
+    simpl (_ ++ _).
+    rewrite IHn.
+    rewrite t2l_cons.
+    reflexivity.
+Qed.
+
+Lemma concat_concat':
+  forall n m (xs: n_tuple bool n) (ys: n_tuple bool m),
+    n_tuple_concat xs ys ~= n_tuple_concat' xs ys.
+Proof.
+  unfold n_tuple_concat.
+  induction m; intros; simpl in *.
+  - destruct ys.
+    simpl in *.
+    revert xs.
+    rewrite <- (plus_zero_trans n).
+    reflexivity.
+  - destruct ys as [ys y]; simpl in *.
+    remember (n_tuple_concat' xs ys) as zs.
+    remember (zs, y) as zsy.
+    change ((n_tuple bool (m + n)%nat * bool)%type) with (n_tuple bool (S m + n)) in zsy.
+    rewrite succ_add_trans.
+    clear Heqzsy Heqzs.
+    generalize (plus_comm_trans n m).
+    revert zs zsy.
+    change (S m + n) with (S (m + n)).
+    generalize (m + n).
+    intros.
+    subst.
+    auto.
+Qed.
+
+Lemma t2l_concat:
+  forall n m (xs: n_tuple bool n) (ys: n_tuple bool m),
+    t2l (n_tuple_concat xs ys) = t2l xs ++ t2l ys.
+Proof.
+  intros.
+  replace (t2l (n_tuple_concat xs ys)) with (t2l (n_tuple_concat' xs ys))
+    by (eapply t2l_proper; symmetry; eapply concat_concat').
+  apply t2l_concat'.
 Qed.
